WIP: Simplify goals

lib/ArithSolver/Basic.lean
@@ -1,28 +1,91 @@
 import Std.Data.HashMap
 import Lean.Meta
+import ArithSolver.Int
 
 open Lean
 open Std (HashMap)
 
+namespace Array
+instance {α} [Hashable α] : Hashable (Array α) where
+  hash
+  | ⟨l⟩ => Hashable.hash l
+
+end Array
+
 namespace ArithSolver
+
+private def intExpr := mkConst ``Int
+
+def intAddExpr : Expr :=
+  let f := mkConst ``HAdd.hAdd [levelZero, levelZero, levelZero]
+  let inst := mkAppN (mkConst ``instHAdd [levelZero]) #[intExpr, mkConst ``Int.instAddInt]
+  mkAppN f #[intExpr, intExpr, intExpr, inst]
+
+def intSubExpr : Expr :=
+  let f := mkConst ``HSub.hSub [levelZero, levelZero, levelZero]
+  let inst := mkAppN (mkConst ``instHAdd [levelZero]) #[intExpr, mkConst ``Int.instSubInt]
+  mkAppN f #[intExpr, intExpr, intExpr, inst]
+
+def intMulExpr : Expr :=
+  let f := mkConst ``HMul.hMul [levelZero, levelZero, levelZero]
+  let inst := mkAppN (mkConst ``instHMul [levelZero]) #[intExpr, mkConst ``Int.instMulInt]
+  mkAppN f #[intExpr, intExpr, intExpr, inst]
+
+def intNegExpr : Expr :=
+  let f := mkConst ``Neg.neg [levelZero]
+  let inst := mkConst ``Int.instNegInt
+  mkAppN f #[intExpr, inst]
+
+-- def intMulExpr : Expr :=
+--   mkApp (mkApp (mkConst ``Mul.mul [levelZero]) intExpr) (mkConst ``Int.instMulInt)
+
+private def intOfNatExpr : Expr := mkConst ``Int.ofNat
+private def intNegSuccExpr : Expr := mkConst ``Int.negSucc
+
+def intNonNegExpr : Expr := mkConst ``Int.NonNeg
+private def intNonNegMkExpr : Expr := mkConst ``Int.NonNeg.mk
+
+-- Create a nat lit as an int
+def natLitAsIntExpr (n:Nat) : Expr :=
+  let z := mkRawNatLit n
+  let ofNat := mkConst ``OfNat.ofNat [levelZero]
+  let inst := mkConst ``Int.instOfNatInt
+  mkAppN ofNat #[intExpr, z, mkApp inst z]
+
+def mkIntLit : Int → Expr
+| Int.ofNat n => natLitAsIntExpr n
+| Int.negSucc n => mkApp intNegExpr (natLitAsIntExpr (n+1))
+
+def intZeroExpr := natLitAsIntExpr 0
 
 def notExpr : Expr := mkConst ``Not
 
-def mkIntEq0Expr (e:Expr) : Expr :=
-  let intZeroExpr : Expr := mkApp (mkConst ``Int.ofNat) (mkLit (Literal.natVal 0))
-  mkAppN (mkConst ``Eq [levelOne]) #[mkConst ``Int, e, intZeroExpr]
+def intEqExpr : Expr := mkApp (mkConst ``Eq [levelOne]) (mkConst ``Int)
 
-def intNonNegExpr : Expr := mkConst ``Int.NonNeg
+def mkIntEq0Expr (e:Expr) : Expr :=
+  mkAppN intEqExpr #[e, intZeroExpr]
 
 def mkIntNonNegExpr (e:Expr) : Expr := mkApp intNonNegExpr e
 
+-- | A variabe
 structure Var where
   (index : UInt32)
-  deriving BEq, Hashable
+  deriving BEq, Hashable, Repr
 
 namespace Var
 
-instance : ToString Var := ⟨λv => toString v.index⟩
+-- | "Variable" that denotes constant one.
+protected def constOne : Var := ⟨0⟩
+
+instance : ToString Var := ⟨λv => "v" ++ toString v.index⟩
+
+instance : Inhabited Var := ⟨Var.constOne⟩
+
+instance : LT Var where
+  lt a b := LT.lt a.index b.index
+
+instance (a b : Var) : Decidable (LT.lt a b) :=
+  inferInstanceAs (Decidable (LT.lt a.index b.index))
 
 end Var
 
@@ -40,39 +103,256 @@ structure Poly where
   -- Poly should be a sorted array of non-zero integers and variable pairs.
   -- The
   elements : Array (Int × Var)
+  deriving BEq, Hashable, Repr
+
+namespace Poly
+
+
+def scalarProd (f:Var → Expr) : Int × Var → Expr
+| (m,  v) => mkAppN intMulExpr #[mkIntLit m, f v]
+
+def firstScalarProd (f: Var → Expr) : Int × Var → Expr
+| (m, ⟨0⟩) => mkIntLit m
+| p => scalarProd f p
+
+-- | Create polynomial denoting constant zero.
+def zero : Poly := ⟨#[]⟩
+
+instance : Inhabited Poly := ⟨zero⟩
+
+-- | Create polynomial denoting constant zero.
+def one : Poly := ⟨#[(1, Var.constOne)]⟩
+
+-- | @add p i _ v@ returns poly denoting @p + i*v@.
+def add : ∀(p:Poly) (m:Int), Var → Poly
+| ⟨a⟩, q, v =>
+  let rec loop : ∀(i : Nat), Poly
+      | 0 => ⟨a.insertAt 0 (q, v)⟩
+      | Nat.succ i =>
+        let (p,u) := a[i]
+        if u < v then
+          ⟨a.insertAt (i+1) (q,v)⟩
+        else if v < u then
+          loop i
+        else -- v = u
+          let q := p+q
+          if q = 0 then
+            ⟨a.eraseIdx i⟩
+          else
+            ⟨a.set! i (q,v)⟩
+  loop a.size
+
+--theorem zero_mv : 0 + m*v =
+
+-- | Map polynomial to expression given mapping from variables
+-- to expressions.
+def buildExpr (f:Var → Expr) (e:Expr) (poly:Subarray (Int × Var)) : Expr := Id.run do
+  let mut e := e
+  for p in poly do
+    e := mkAppN intAddExpr #[e, scalarProd f p]
+  pure e
+
+-- | Map polynomial to expression given mapping from variables
+-- to expressions.
+def expr (f:Var → Expr) : Poly → Expr
+| ⟨#[]⟩ => intZeroExpr
+| ⟨a⟩ => buildExpr f (firstScalarProd f a[0]) a[1:]
+
+
+theorem buildProofLemma {x c a:Int} (h:x + c = a) (y:Int)
+  : (x + y) + c = a + y := sorry
+
+-- buildProof f x c a h rest where h is a proof of "x + c = a" returns
+-- a proof "buildExpr f x rest + c = buildExpr f a rest"
+def buildProof (f:Var → Expr) (x c a h :Expr) (rest:Subarray (Int × Var)) : Expr := Id.run do
+  let mut x := x
+  let mut a := a
+  let mut h := h
+  for p in rest do
+    let y := scalarProd f p
+    h := mkAppN (mkConst ``buildProofLemma) #[x,c, a, h, y]
+    x := mkAppN intAddExpr #[x, y]
+    a := mkAppN intAddExpr #[a, y]
+  pure h
+
+
+-- | Map polynomial to expression given mapping from variables
+-- to expressions.
+def sexpr (f:Var → Expr) (a:Array (Int × Var)) (i:Nat) : Expr :=
+  if i = 0 then
+    intZeroExpr
+  else
+    buildExpr f (firstScalarProd f a[0]) a[1:i]
+
+theorem sum0Lemma (p q v:Int) : p*v + q*v = (p+q)*v := Eq.symm (Int.add_mul _ _ _)
+
+theorem sumLemma (r p q v:Int) : (r + p*v) + q*v = r + (p+q)*v := by
+  apply Eq.trans (Int.add_assoc r _ _)
+  apply congrArg (fun y => r + y)
+  exact sum0Lemma _ _ _
+
+-- @mkSum0Proof f p q v@ with "p + q ≠ 0" produces a proof that
+--   firstScalarProd f (p,v) + firstScalarProd (q,v) = firstScalarProd f (p+q, v)
+def mkSum0Proof (f : Var → Expr) (p q:Int) (v:Var) : Expr :=
+  mkAppN (mkConst ``sum0Lemma) #[ mkIntLit p, mkIntLit q, f v]
+
+-- @mkSumProof f poly i p q v@ with "p + q ≠ 0" and i > 0 produces a proof that
+--   expr f ⟨poly[0:i].toArray.push (p,v)⟩ + firstScalarProd (q,v) = expr f ⟨poly[0:i].toArray.push (p+q, v)⟩
+def mkSumProof (f : Var → Expr) (poly:Array (Int × Var)) (i:Nat) (p q:Int) (v:Var) : Expr :=
+  let r := sexpr f poly i
+  mkAppN (mkConst ``sumLemma) #[r, mkIntLit p, mkIntLit q, f v]
+
+theorem cancel0Lemma {p q:Int} (h : p+q = 0) (v:Int) : p*v + q*v = 0 := by
+  apply Eq.trans (sum0Lemma p q v)
+  exact @Eq.substr Int (λx => x * v = 0) _ _ h (Int.zero_mul v)
+
+example        : (64:Int) + -64 = 0   := @cancel0Lemma (64) (-64) (@rfl Int 0) 1
+example        : (-64:Int) + 64 = 0   := @cancel0Lemma (-64) (64) (@rfl Int 0) 1
+example (v:Int): -64 * v + 64 * v = 0 := @cancel0Lemma (-64) 64   (@rfl Int 0) v
+example (v:Int): 64 * v + -64 * v = 0 := @cancel0Lemma (64) (-64) (@rfl Int 0) v
+
+-- @mkCancel0Proof f q v@ produces a proof that
+--  firstScalarProd f (-q,v) + firstScalarProd (q,v) = intZeroExpr
+def mkCancel0Proof (f : Var → Expr) (q:Int) (v:Var) : Expr :=
+  let rflExpr := mkAppN (mkConst ``rfl [levelOne]) #[intExpr, intZeroExpr]
+  mkAppN (mkConst ``cancel0Lemma) #[ mkIntLit (-q), mkIntLit q, rflExpr, f v]
+
+theorem cancelLemma (r p q v:Int) (h : p+q = 0) : (r + p*v) + q*v = r := by
+  apply Eq.trans (Int.add_assoc r _ _)
+  exact Eq.trans (cancel0Lemma h v ▸ rfl) (Int.add_zero r)
+
+
+-- @mkCancelProof f poly i q v@ with i > 0 produces a proof that
+--  (expr f poly[0:i] + -q * v⟩) + scalarProd (q,v) = sexpr f poly[0:i]
+def mkCancelProof (f : Var → Expr) (poly:Array (Int × Var)) (i:Nat) (q:Int) (v:Var) : Expr :=
+  let r := sexpr f poly i
+  let rflExpr := mkAppN (mkConst ``rfl [levelOne]) #[intExpr, intZeroExpr]
+  mkAppN (mkConst ``cancelLemma) #[r, mkIntLit (-q), mkIntLit q, f v, rflExpr]
+
+-- | @addProof f p m v@ returns proof showing that
+-- @p.expr + firstScalarProd f (m, v) = (p.add m v).expr@.
+def addProof (f:Var → Expr) : ∀(poly:Poly) (q:Int), q ≠ 0 → Var → Expr
+| ⟨poly⟩, q, g, v =>
+  let c := firstScalarProd f (q,v)
+  let rec loop : ∀(i : Nat), Expr
+      | 0 =>
+        if poly.size = 0 then
+          -- Prove (0:Int) + firstScalarProd f (q,v) = firstScalarProd f (q,v)
+          mkApp (mkConst `Int.zero_add) c
+        else Id.run do
+          let x := scalarProd f poly[0]
+          let a := mkAppN intAddExpr #[c, x]
+          let h := mkAppN (mkConst `Int.add_comm) #[x, c]
+          buildProof f x c a h poly[1:]
+      | Nat.succ i =>
+        let (p,u) := poly[i]
+        if u < v then
+          let x := buildExpr f (firstScalarProd f poly[0]) poly[1:i+1]
+          let a := mkAppN intAddExpr #[x, c]
+          let h := mkAppN (mkConst ``Eq.refl [levelOne]) #[intExpr, a]
+          buildProof f x c a h poly[i+1:]
+        else if v < u then
+          loop i
+        else -- v = u
+          if p+q = 0 then
+            if i = 0 then
+              let a := intZeroExpr
+              let x := firstScalarProd f poly[0]
+              let h := mkCancel0Proof f q v
+              buildProof f x c a h poly[i+1:]
+            else
+              let a := sexpr f poly i
+              let x := mkAppN intAddExpr #[a, scalarProd f poly[i]]
+              let h := mkCancelProof f poly i q v
+              buildProof f x c a h poly[i+1:]
+          else
+            if i = 0 then
+              let x := firstScalarProd f poly[0]
+              let a := firstScalarProd f (p+q, v)
+              let h := mkSum0Proof f p q v
+              buildProof f x c a h poly[i+1:]
+            else
+              let x0 := sexpr f poly i
+              let x := mkAppN intAddExpr #[x0, scalarProd f poly[i]]
+              let a := mkAppN intAddExpr #[x0, scalarProd f (p+q, v)]
+              let h := mkSumProof f poly i p q v
+              buildProof f x c a h poly[i+1:]
+  loop poly.size
+
+protected def toString : Poly → String
+| ⟨a⟩ =>
+  let scalarProd : Int × Var → String
+--          | (1, v) => varExpr s v
+--          | (-1, v) => mkApp intNegExpr (varExpr s v)
+        | (m,v) => s!"{m}*{v}"
+  let firstScalarProd : Int × Var → String
+        | (m, ⟨0⟩) => toString m
+        | p => scalarProd p
+  let polyIns := λ(e:String) h => s!"{e} + {scalarProd h}"
+  a[1:].foldl polyIns (firstScalarProd a[0])
+
+instance : ToString Poly where
+  toString := Poly.toString
+
+end Poly
 
 -- | Identifies the origin of an assertion
-inductive Origin
+inductive Assertion.Origin
 -- | A local context with the given name, user name and the new name.
 | localContext : FVarId → Name → FVarId → Origin
+-- Assertion came from negating a goal with proofs using the new name
 | negGoal : FVarId → Origin
+-- Assertion came from a natural number from an uninterpreted declaration.
 | uninterpNat : Origin
 
+-- | Assertion added
 structure Assertion where
-  origin : Origin
+  origin : Assertion.Origin
   proof : Expr
   prop : Pred
 
-def int1Lit : Expr := mkApp (mkConst ``Int.ofNat) (mkLit (Literal.natVal 1))
+-- def int1Lit : Expr := mkApp (mkConst ``Int.ofNat) (mkLit (Literal.natVal 1))
+
+-- Definition associated with a variable.
+inductive Decl
+| uninterp : Expr → Decl
+| poly : Poly → Decl
+deriving BEq, Hashable
+
+namespace Decl
+
+protected def toString : Decl → String
+| uninterp e => s!"uninterp {e}"
+| poly p => s!"poly {p}"
+
+instance : ToString Decl where
+  toString := Decl.toString
+
+instance : Inhabited Decl := ⟨uninterp arbitrary⟩
+
+end Decl
 
 structure State where
   -- Map from expressions (which should have type 'Int') to the theor
   -- variable associated with it.
-  exprMap : HashMap Expr Var := Std.mkHashMap
+  exprMap : HashMap Decl Var := Std.mkHashMap
   -- Map from variables (which should have type 'Int') to the expression
   -- associated with it.
-  varExprs : Array Expr := #[int1Lit]
+  varExprs : Array Decl := #[Decl.poly Poly.one]
   -- Predicates asserted to be true.
   assertions : Array Assertion := #[]
 
 namespace State
 
-def varExpr (s:State) (v:Var) : Expr := s.varExprs.get! v.index.toNat
+partial def varExpr (s:State) (v:Var) : Expr :=
+  match s.varExprs.get! v.index.toNat with
+  | Decl.uninterp e => e
+  | Decl.poly p => p.expr (varExpr s)
 
 def predExpr (s:State) : Pred → Expr
 | Pred.IsEq0 v => mkIntEq0Expr (s.varExpr v)
 | Pred.IsNe0 v => mkApp notExpr (mkIntEq0Expr (s.varExpr v))
-| Pred.IsGe0 v => mkIntNonNegExpr (s.varExpr v)
+| Pred.IsGe0 v => mkApp intNonNegExpr (s.varExpr v)
 
 end State
 
@@ -82,24 +362,68 @@ abbrev ArithM  := StateRefT State MetaM
   StateRefT'.run m s
 
 -- | Return a theory variable associated with the given uninterpreted Lean expression.
-def getUninterpVar (e:Expr) : ArithM Var := do
+def mkDeclVar (d:Decl) : ArithM Var := do
   let s ← get
-  match s.exprMap.find? e with
+  match s.exprMap.find? d with
   | none => pure ()
   | some v => return v
+  IO.println $ s!"Creating variable {d}"
   let newVar := ⟨OfNat.ofNat s.varExprs.size⟩
-  let newExprMap  := s.exprMap.insert e newVar
-  let newVarExprs := s.varExprs.push e
+  let newExprMap  := s.exprMap.insert d newVar
+  let newVarExprs := s.varExprs.push d
   if (OfNat.ofNat s.varExprs.size : UInt32) = 0 then
     throwError m!"Arithmetic variable overflow."
   set { s with exprMap := newExprMap, varExprs := newVarExprs }
   return newVar
 
+-- | Return a theory variable associated with the given uninterpreted Lean expression.
+def getUninterpVar (e:Expr) : ArithM Var := do
+  mkDeclVar (Decl.uninterp (← Meta.instantiateMVars e))
 
 -- | Assert a predicate holds using the given expression to refer to the
 -- proof.
-def assertPred (origin:Origin) (proof:Expr) (prop:Pred) : ArithM Unit := do
+def assertPred (origin:Assertion.Origin) (proof:Expr) (prop:Pred) : ArithM Unit := do
   let a := { origin := origin, proof := proof, prop := prop }
   modifyGet fun s => ((), { s with assertions := s.assertions.push a })
+
+-- @polyAddProof s poly q _ v@ returns a proof that
+--   @poly.expr varExpr s + firstScalarProd s.varExpr (m, v) = (poly.add m v).expr s.varExpr@.
+def varAddProof (poly:Poly) (q:Int) (q_ne:q ≠ 0) (v:Var) : ArithM Expr := do
+  let s ← get
+  pure $ Poly.addProof (s.varExpr) poly q q_ne v
+
+
+-- @polyAddProof s poly q _ v@ returns a proof that
+--   @poly.expr varExpr s + firstScalarProd s.varExpr (m, v) = (poly.add m v).expr s.varExpr@.
+def polyAddProof (poly:Poly) (q:Int) (q_ne:q ≠ 0) (v:Var) : ArithM Expr := do
+  let s ← get
+  pure $ Poly.addProof (s.varExpr) poly q q_ne v
+
+
+/-
+structure Equiv where
+  -- New type representation
+  newInt : Expr
+  -- An equality
+  eqProof : Expr
+
+def Poly.mkEquiv : Poly → MetaM Equiv := sorry
+
+-- structure PolyV (v:Int) where
+--  sorry : Int
+
+def processAdd (p m u v a b : Int)
+  (g: p + m * u = a)
+  (h: a + m * v = b)
+  : p + m * (u+v) = b := sorry
+
+def processSub (p m u v a b : Int)
+  (g: p + m * u = a)
+  (h: a + (-m) * v = b)
+  : p + m * (u-v) = b := sorry
+
+-- def pushLeftAdd (z x y : Int) : BinPoly z m (x + y) → BinPoly z m x
+-/
+
 
 end ArithSolver
