lib/ArithSolver/Int.lean
@@ -29,7 +29,7 @@ theorem zero_add (x : Int) : 0 + x = x :=
   | negSucc n => rfl
 
 theorem sub_add_neg (x : Int) : x - y = x + -y := by rfl
-    
+
 theorem negOfNat_zero : negOfNat 0 = 0 := by rfl
 
 theorem negOfNat_succ : negOfNat (Nat.succ n) = negSucc n := by rfl
@@ -51,34 +51,34 @@ theorem neg_subNatNat (m n: Nat) : - (subNatNat m n) = subNatNat n m := by
       simp
     | succ n =>
       simp [neg_negSucc, Nat.add_succ, sub_add_neg, negOfNat_zero, Nat.zero_sub]
-  | succ m => 
-    simp [HSub.hSub, Sub.sub, Int.sub]    
+  | succ m =>
+    simp [HSub.hSub, Sub.sub, Int.sub]
     simp [neg_ofNat, negOfNat_succ]
-    simp [HAdd.hAdd, Add.add, Int.add]    
+    simp [HAdd.hAdd, Add.add, Int.add]
     simp [subNatNat]
     generalize g:n-m.succ=n_sub_m
     cases n_sub_m with
-    | zero => 
+    | zero =>
       simp [neg_ofNat]
       generalize m.succ-n=m_sub_n
       cases m_sub_n with
-      | zero => 
-        simp [negOfNat_succ]        
+      | zero =>
+        simp [negOfNat_succ]
       | succ m_sub_n =>
         simp [negOfNat_succ]
     | succ n_sub_m =>
       generalize h:m.succ-n=m_sub_n
       cases m_sub_n with
-      | zero => 
+      | zero =>
         simp [neg_negSucc]
       | succ m_sub_n =>
         have r : Nat.succ m ≤ n:= Nat.le_of_lt (Nat.lt_of_sub_succ g)
         have s : ¬ (Nat.succ m ≤ n) := Nat.not_le_of_gt (Nat.lt_of_sub_succ h)
         exact False.elim (s r)
 
-theorem neg_add (x y : Int) : -(x + y) = -x + -y := 
+theorem neg_add (x y : Int) : -(x + y) = -x + -y :=
   match x, y with
-  | 0, y => by 
+  | 0, y => by
     simp only [Int.zero_add, Int.neg_zero]
   | ofNat (Nat.succ x), ofNat 0 => by rfl
   | ofNat (Nat.succ x), ofNat (Nat.succ y) => by
@@ -93,7 +93,8 @@ theorem neg_add (x y : Int) : -(x + y) = -x + -y :=
     simp only [negSucc_add_negSucc, neg_negSucc, ofNat_add_ofNat]
     simp only [Nat.add_succ, Nat.succ_add, Nat.add_zero]
 
-theorem ofNat_add_subNatNat (x y z:Nat) 
+private
+theorem ofNat_add_subNatNat (x y z:Nat)
   : ofNat x + subNatNat y z = subNatNat (x + y) z := by
     simp [subNatNat]
     generalize g: z - y = z_sub_y
@@ -105,7 +106,7 @@ theorem ofNat_add_subNatNat (x y z:Nat)
       rw [Nat.add_comm y x]
       apply Nat.add_sub
       exact (Nat.sub_is_zero_is_le.mpr g)
-    | succ j => 
+    | succ j =>
       simp [ofNat_add_negSucc, subNatNat]
       simp [g.symm]
       rw [Nat.add_comm x y, Nat.sub_sub_lassoc]
@@ -113,18 +114,88 @@ theorem ofNat_add_subNatNat (x y z:Nat)
       have r := Nat.sub_sub_rassoc x p
       rw [r, Nat.add_comm y x]
 
+private
 theorem subNatNat_add_ofNat (x y z:Nat) : subNatNat x y + ofNat z = subNatNat (x + z) y := by
-  admit
+  simp [subNatNat]
+  generalize g:y-x=j
+  cases j with
+  | zero =>
+    have q : y <= x := Nat.sub_is_zero_is_le.mpr g
+    simp [Eq.symm (Nat.sub_sub_lassoc _ _ _), g, Nat.zero_sub, ofNat_add_ofNat,
+          Nat.sub_add_lassoc _ q]
+  | succ j =>
+    simp [negSucc_add_ofNat, subNatNat, g.symm]
+    have q := Nat.sub_sub_lassoc y x z
+    have h : x ≤ y := Nat.le_of_lt (Nat.lt_of_sub_succ g)
+    have r := Nat.sub_sub_rassoc z h
+    have s := Nat.add_comm z x
+    simp [q, r, s]
 
-theorem negSucc_add_subNatNat (x y z:Nat) : negSucc x + subNatNat y z = subNatNat y (Nat.succ (x + z)) := sorry
-theorem subNatNat_add_negSucc (x y z:Nat) : subNatNat x y + negSucc z = subNatNat x (Nat.succ (y + z)) := sorry
+theorem negSucc_add_subNatNat (x y z:Nat) : negSucc x + subNatNat y z = subNatNat y (Nat.succ (x + z)) := by
+  simp [subNatNat]
+  generalize g:z-y=j
+  cases j with
+  | zero =>
+    simp [negSucc_add_ofNat, subNatNat]
+    have h : z ≤ y := Nat.sub_is_zero_is_le.mpr g
+    have p := Nat.sub_sub_rassoc (Nat.succ x) h
+    have q := Nat.sub_sub_lassoc
+    have r := Nat.add_comm z (Nat.succ x)
+    simp [p, Nat.succ_add, q, r]
+  | succ j =>
+    rw [negSucc_add_negSucc]
+    have p : Nat.succ (x + j) = x + (z- y) := by
+      simp [(Nat.add_succ _ _).symm, g.symm]
+    rw [p]
+    have q :  Nat.succ (x + z) - y = Nat.succ (x + (z - y)) := by
+      have h : y ≤ z := Nat.le_of_lt (Nat.lt_of_sub_succ g)
+      have h2 : y ≤ x + z := Nat.le_trans h (Nat.le_add_left z x)
+      simp [Nat.add_sub _ h, Nat.succ_sub h2]
+    simp [q]
+
+theorem subNatNat_add_negSucc (x y z:Nat)
+  : subNatNat x y + negSucc z = subNatNat x (Nat.succ (y + z)) := by
+  simp [subNatNat]
+  generalize g:y-x=j
+  cases j with
+  | zero =>
+    simp [ofNat_add_negSucc, subNatNat]
+    have g : Nat.succ z - (x - y) = Nat.succ (y + z) - x := by
+      have h : y ≤ x := Nat.sub_is_zero_is_le.mpr g
+      have p := Nat.sub_sub_rassoc (Nat.succ z) h
+      simp [p, Nat.succ_add, Nat.add_comm z y]
+    have h : x - y - Nat.succ z = x - Nat.succ (y + z) := by
+      simp [Nat.sub_sub_lassoc, Nat.add_succ]
+    simp [g, h]
+  | succ j =>
+    simp [negSucc_add_negSucc]
+    have p : x ≤ y := Nat.le_of_lt (Nat.lt_of_sub_succ g)
+    have h : Nat.succ (y + z) - x = Nat.succ ((y+z) - x) := by
+      have q : x ≤ y + z := Nat.le_trans p (Nat.le_add_right y z)
+      have r := Nat.succ_sub q
+      simp [r]
+    simp [h, (Nat.succ_add j z).symm, g.symm]
+    have q := @Nat.sub_add_lassoc y x z p
+    exact q
+
+theorem add_comm (x y : Int) : x + y = y + x := by
+  cases x <;> cases y <;> simp only
+    [ofNat_add_ofNat, ofNat_add_negSucc,
+     negSucc_add_ofNat, negSucc_add_negSucc,
+     Nat.add_comm]
 
 theorem add_assoc (x y z : Int) : x + y + z = x + (y + z) := by
-  cases x <;> cases y <;> cases z <;>  simp only 
+  cases x <;> cases y <;> cases z <;>  simp only
     [ofNat_add_ofNat, ofNat_add_negSucc, negSucc_add_ofNat, negSucc_add_negSucc,
       ofNat_add_subNatNat, subNatNat_add_ofNat,
       subNatNat_add_negSucc, negSucc_add_subNatNat,
       Nat.succ_add, Nat.add_succ, Nat.add_assoc]
+
+theorem zero_mul (x:Int) : 0 * x = 0 := sorry
+
+theorem one_mul (x:Int) : 1 * x = x := sorry
+
+theorem add_mul (n m k : Int) : (n + m) * k = n * k + m * k := sorry
 
 -- This section contains theorems that turn comparisons into normal forms.
 section predicateToNonNeg
@@ -132,7 +203,7 @@ section predicateToNonNeg
 theorem nonNeg_of_le {x y : Int} (p : x ≤ y) : NonNeg (y + -x) := p
 
 theorem nonNeg_of_lt {x y : Int} (p : x < y) : NonNeg (y + -x + -1) := by
-  have q := nonNeg_of_le p 
+  have q := nonNeg_of_le p
   simp [neg_add, (add_assoc _ _ _).symm] at q
   exact q
 
@@ -140,26 +211,26 @@ theorem nonNeg_of_ge {x y : Int} (p : x ≥ y) : NonNeg (x + -y) := p
 
 theorem nonNeg_of_gt {x y : Int} (p : x > y) : NonNeg (x + -y + -1) := nonNeg_of_lt p
 
-theorem nonNeg_of_le_Nat {m n : Nat} (p : m ≤ n) : NonNeg (ofNat n + -ofNat m) := by  
+theorem nonNeg_of_le_Nat {m n : Nat} (p : m ≤ n) : NonNeg (ofNat n + -ofNat m) := by
   cases m with
   | zero =>
     exact NonNeg.mk n
-  | succ m => 
+  | succ m =>
     simp only [neg_ofNat, negOfNat_succ]
     simp only [HAdd.hAdd, Add.add, Int.add]
     have q := Nat.sub_is_zero_is_le.mp p
     simp only [subNatNat, q]
     exact NonNeg.mk _
 
-theorem nonNeg_of_lt_Nat {m n : Nat} (p : m < n) : NonNeg (ofNat n + -ofNat m + -1) := by  
-  have q := nonNeg_of_le_Nat p 
+theorem nonNeg_of_lt_Nat {m n : Nat} (p : m < n) : NonNeg (ofNat n + -ofNat m + -1) := by
+  have q := nonNeg_of_le_Nat p
   simp only [ofNat_succ, neg_add] at q
   simp only [add_assoc, q]
 
-theorem nonNeg_of_ge_Nat {x y : Nat} (p : x ≥ y) : NonNeg (ofNat x + -ofNat y) := 
+theorem nonNeg_of_ge_Nat {x y : Nat} (p : x ≥ y) : NonNeg (ofNat x + -ofNat y) :=
   nonNeg_of_le_Nat p
 
-theorem nonNeg_of_gt_Nat {x y : Nat} (p : x > y) : NonNeg (ofNat x + -ofNat y + -1) := 
+theorem nonNeg_of_gt_Nat {x y : Nat} (p : x > y) : NonNeg (ofNat x + -ofNat y + -1) :=
   nonNeg_of_lt_Nat p
 
 end predicateToNonNeg
