lib/ArithSolver/Nat.lean
@@ -1,16 +1,16 @@
 namespace Nat
 
 protected
-theorem zero_sub (n : Nat) : 0 - n = 0 := by 
+theorem zero_sub (n : Nat) : 0 - n = 0 := by
   induction n with
   | zero => rfl
   | succ n ind => simp [sub_succ, ind]
 
 protected
-theorem sub_is_zero_is_le {m n : Nat} : m ≤ n ↔ m - n = 0 := by 
+theorem sub_is_zero_is_le {m n : Nat} : m ≤ n ↔ m - n = 0 := by
   revert m
   induction n with
-  | zero => 
+  | zero =>
     intros m
     cases m with
     | zero =>
@@ -19,10 +19,10 @@ theorem sub_is_zero_is_le {m n : Nat} : m ≤ n ↔ m - n = 0 := by
       simp
       intro p
       cases p
-  | succ n ind => 
+  | succ n ind =>
     intros m
     cases m with
-    | zero => 
+    | zero =>
       simp [Nat.zero_sub, Nat.zero_le]
     | succ m =>
       simp [succ_sub_succ]
@@ -32,36 +32,16 @@ theorem sub_is_zero_is_le {m n : Nat} : m ≤ n ↔ m - n = 0 := by
       case succ.succ.mpr =>
         exact λp => Nat.succ_le_succ (ind.mpr p)
 
-/-
-protected
-theorem sub_is_zero_of_le {m n : Nat} (p:m ≤ n) : m - n = 0 := by 
-  revert m
-  induction n with
-  | zero => 
-    intros m p
-    cases m with
-    | zero => exact (Nat.zero_sub _)
-    | succ m => 
-      cases p
-  | succ n ind => 
-    intros m p
-    cases m with
-    | zero => exact (Nat.zero_sub _)
-    | succ m =>
-      simp [succ_sub_succ]
-      exact (ind (Nat.le_of_succ_le_succ p))
--/
-
 theorem lt_of_sub_succ {n m k:Nat} (p:n - m = Nat.succ k) : m < n := by
   revert n
   induction m with
-  | zero => 
+  | zero =>
     intros n p
     simp at p
     simp [p]
     exact Nat.succ_le_succ (Nat.zero_le _)
   | succ m ind =>
-    intros n p 
+    intros n p
     cases n with
     | zero =>
       simp [Nat.zero_sub] at p
@@ -69,13 +49,24 @@ theorem lt_of_sub_succ {n m k:Nat} (p:n - m = Nat.succ k) : m < n := by
       simp [succ_sub_succ] at p
       exact Nat.succ_lt_succ (ind p)
 
+
+-- These theorems are intended to rewrite to a mixture of additions and
+-- subtractions into one sum minus another sum.
+
 theorem sub_sub_lassoc (x y z:Nat) : x - y - z = x - (y + z) := by
   admit
 
 theorem sub_sub_rassoc (x:Nat) {y z:Nat} (p:y >= z) : x - (y - z) = x + z - y := by
   admit
 
+theorem sub_add_lassoc {x y:Nat} (z:Nat) (p:x >= y) : x - y + z = x + z - y := by
+  admit
+
 theorem add_sub (x:Nat) {y z:Nat} (p:y >= z) : x + (y - z) = x + y - z := by
+  admit
+
+protected
+theorem succ_sub {x y :Nat} (p:y ≤ x) : Nat.succ (x - y) = Nat.succ x - y := by
   admit
 
 end Nat
